refactor: simple context

LeanMlirCommon/SimplyTyped/Context.lean
@@ -1,4 +1,5 @@
 import LeanMlirCommon.UnTyped.Basic
+import Std.Data.List.Lemmas
 
 namespace MLIR.SimplyTyped
 
@@ -11,12 +12,24 @@ namespace Context
 def hasType (Γ : Context Ty) (v : VarName) (ty : Ty) : Prop :=
   Γ.lookup v = some ty
 
-/-- `Γ.push v ty` returns a context which maps `v` to `ty`, and works like `Γ` on all other
-variables -/
-def push (Γ : Context Ty) (v : VarName) (ty : Ty) :=
-  (v, ty) :: Γ
-
 /-- `Γ.hasType v ty` is decidable when our type universe has decidable equality -/
 instance {Γ : Context Ty} [DecidableEq Ty] {v ty} :
     Decidable (Γ.hasType v ty) := by
   unfold hasType; infer_instance
+
+/-- `Γ.push v ty` returns a context which maps `v` to `ty`, and works like `Γ` on all other
+variables -/
+def push (Γ : Context Ty) (v : VarName) (ty : Ty) : Context Ty :=
+  (v, ty) :: Γ
+
+/-- Two contexts are extensionally equal if they map each variable to the same type -/
+def ExtEq (Γ Δ : Context Ty) : Prop :=
+  ∀ v, Γ.lookup v = Δ.lookup v
+
+@[simp] theorem hasType_push {Γ : Context Ty} :
+    (Γ.push v ty).hasType v ty := by
+  simp [push, hasType]
+
+@[simp] theorem hasType_push_of_neq {Γ : Context Ty} (h : w ≠ v) :
+    (Γ.push v ty).hasType w ty' ↔ Γ.hasType w ty' := by
+  simp [push, hasType, List.lookup, (beq_eq_false_iff_ne _ _).mpr h]
